Simple_Clause_Learning/Simple_Clause_Learning.thy
@@ -2177,6 +2177,27 @@ qed
 lemma finite_lits_less_eq_B: "finite {L. atm_of L \<prec>\<^sub>B \<beta> \<or> atm_of L = \<beta>}"
   using finite_lits_less_B by (simp add: lits_less_eq_B_conv)
 
+lemma Collect_ball_eq_Pow_Collect: "{X. \<forall>x \<in> X. P x} = Pow {x. P x}"
+  by blast
+
+lemma finite_lit_clss_nodup_less_B: "finite {C. \<forall>L \<in># C. atm_of L \<prec>\<^sub>B \<beta> \<and> count C L = 1}"
+proof -
+  have 1: "(\<forall>L \<in># C. P L \<and> count C L = 1) \<longleftrightarrow> (\<exists>C'. C = mset_set C' \<and> finite C' \<and> (\<forall>L \<in> C'. P L))"
+    for C P
+    by (smt (verit) count_eq_zero_iff count_mset_set' finite_set_mset finite_set_mset_mset_set
+        multiset_eqI)
+
+  have 2: "finite {C'. \<forall>L\<in>C'. atm_of L \<prec>\<^sub>B \<beta>}"
+    unfolding Collect_ball_eq_Pow_Collect finite_Pow_iff
+    by (rule finite_lits_less_B)
+
+  show ?thesis
+    unfolding 1
+    unfolding setcompr_eq_image
+    apply (rule finite_imageI)
+    using 2 by simp
+qed
+
 
 subsection \<open>Rules\<close>
 
@@ -4016,6 +4037,12 @@ proof (cases N \<beta> S1 S2 rule: conflict.cases)
     thus ?thesis by simp
   qed
 qed
+
+lemma ball_less_B_if_trail_false_and_trail_atoms_lt:
+  "trail_false_cls (state_trail S) C \<Longrightarrow> trail_atoms_lt \<beta> S \<Longrightarrow> \<forall>L \<in># C. atm_of L \<prec>\<^sub>B \<beta>"
+  unfolding trail_atoms_lt_def
+  by (meson atm_of_in_atm_of_set_iff_in_set_or_uminus_in_set trail_false_cls_def
+      trail_false_lit_def)
 
 
 section \<open>Soundness\<close>
